HashTable/hashtbl_proof_manual.v
@@ -72,15 +72,10 @@ Proof. Admitted.
 Lemma proof_of_hashtbl_remove_which_implies_wit_1 : hashtbl_remove_which_implies_wit_1.
 Proof. Admitted. 
 
-Lemma proof_of_hashtbl_free_blist_return_wit_1 : hashtbl_free_blist_return_wit_1.
-Proof. pre_process. entailer!. Admitted. 
-
 Lemma proof_of_hashtbl_free_blist_return_wit_2 : hashtbl_free_blist_return_wit_2.
 Proof. pre_process. entailer!. rewrite H.
   sep_apply sll_zero.
   - entailer!. 
-  simpl.
-  entailer!.
   - entailer!.
 Qed. 
 
@@ -126,6 +121,8 @@ Exists l_2.
 Exists lh_2.
 Exists b_2.
 entailer!.
+sep_apply (store_map_missing_i_equiv_store_map_first_i store_sll b_2).
+entailer!.
 Qed.
  
 
@@ -140,8 +137,10 @@ Proof. pre_process.
       (* sepcon_lift (PtrArray.missing_i h_pre_bucks_3 i 0 211 lh_2).
       sepcon_lift ((h_pre_bucks_3 + i * sizeof ( PTR )) # Ptr |-> 0).
       sep_apply (PtrArray.missing_i_merge_to_full h_pre_bucks_3 i 211 0 lh_2). *)
-      sepcon_lift (store_map_missing_i store_sll b_2 i).
-      sep_apply (store_map_merge store_sll i (buck_i_2, nil) b_2).
+      (* sepcon_lift (store_map_missing_first_i_Z store_sll b_2 i).
+      sep_apply (store_map_missing_first_i_split store_sll i ((h_pre_bucks_3 + (i+1) * sizeof ( PTR )), nil) b_2).
+      sepcon_lift (store_sll i (h_pre_bucks_3 + (i+1) * sizeof ( PTR ), nil)).
+      unfold store_sll. *)
       (* 2:{ specialize (H6 i buck_i_2). admit. } *)
       sepcon_lift (PtrArray.missing_i h_pre_bucks_3 i 0 211 lh_2).
       sepcon_lift ((h_pre_bucks_3 + i * sizeof ( PTR )) # Ptr |-> 0).
@@ -151,15 +150,19 @@ Proof. pre_process.
       (* assert ((replace_Znth i 0 lh_2) = lh_2).
       {admit. } *)
       2:{ lia. }
-      assert (0 <= i < Zlength lh_2) by (rewrite Zlength_correct; lia ).
-      specialize (H6 i (Znth i lh_2 0)).
+      assert (0 <= (i+1) < Zlength lh_2) by (rewrite Zlength_correct; lia ).
+      specialize (H6 (i+1) (Znth (i+1) lh_2 0)).
       destruct H6 as [H6_left H6_right].
-      assert (0 <= i < Zlength lh_2 /\ Znth i lh_2 0 = Znth i lh_2 0).
-      { split; [exact H11|reflexivity]. }
-      assert (exists l : list addr, b_2 i = Some (Znth i lh_2 0, l)) as Hex.
+      assert (0 <= (i+1) < Zlength lh_2 /\ Znth (i+1) lh_2 0 = Znth (i+1) lh_2 0).
+      { split; [exact H10|reflexivity]. }
+      assert (exists l : list addr, b_2 (i+1) = Some (Znth (i+1) lh_2 0, l)) as Hex.
       {apply H6_right. exact H6. }
       destruct Hex as [li Hb].
-      2:{ specialize (H6 i buck_i_2). admit. }
+      sepcon_lift (store_map_missing_first_i_Z store_sll b_2 i).
+      sep_apply (store_map_missing_first_i_split store_sll i (Znth (i + 1) lh_2 0, li) b_2).
+      2:{ exact Hb. }
+      sepcon_lift (store_sll i (Znth (i + 1) lh_2 0, li)).
+      unfold store_sll.
       prop_apply PtrArray.full_length.  (* 获取Zlength lh_2 = 211 *)
       entailer!.
       assert (0 <= (i+1) < Zlength lh_2) by (rewrite Zlength_correct; lia ).
@@ -173,14 +176,14 @@ Proof. pre_process.
       destruct Hex_2 as [li_2 Hb_2].
 
       (* 现在我们知道b 0 = Some (buck, li)，其中buck = Znth 0 lh_2 0 *)
-      sep_apply (store_map_split store_sll (i+1) (Znth (i+1) lh_2 0, li_2) b_2 Hb_2).
+      (* sep_apply (store_map_split store_sll (i+1) (Znth (i+1) lh_2 0, li_2) b_2 Hb_2). *)
 
       (* 从IntArray中提取指针 *)
       sep_apply (PtrArray.full_split_to_missing_i h_pre_bucks_3 (i+1) 211 (replace_Znth i 0 lh_2) 0).
       2: { lia. }
-      sepcon_lift (store_sll (i + 1) (Znth (i + 1) lh_2 0, li_2)).
-      unfold store_sll.
-      Exists li_2.
+      (* sepcon_lift (store_sll (i + 1) (Znth (i + 1) lh_2 0, li_2)).
+      unfold store_sll. *)
+      Exists li.
       Exists (Znth (i + 1) lh_2 0).
       Exists h_pre_bucks_3.
       Exists l_2.
@@ -193,9 +196,9 @@ Proof. pre_process.
       + apply repr_equal. 
         tauto.
     - Left.
-      sepcon_lift (store_map_missing_i store_sll b_2 i).
-      sep_apply (store_map_merge store_sll i (buck_i_2, nil) b_2).
-      2:{ admit. }
+      sep_apply (store_map_missing_first_i_empty store_sll i b_2).
+      2: { lia. }
+      entailer!.
       sepcon_lift (PtrArray.missing_i h_pre_bucks_3 i 0 211 lh_2).
       sepcon_lift ((h_pre_bucks_3 + i * sizeof ( PTR )) # Ptr |-> 0).
       sep_apply (PtrArray.missing_i_merge_to_full h_pre_bucks_3 i 211 0 lh_2).
@@ -205,7 +208,7 @@ Proof. pre_process.
       Exists lh_2.
       Exists b_2.
       entailer!.
-      sep_apply PtrArray.full_replace_nth; [ entailer! | lia ].
+      (* sep_apply PtrArray.full_replace_nth; [ entailer! | lia ]. *)
  Admitted.  
 
 Lemma proof_of_hashtbl_clear_which_implies_wit_1 : hashtbl_clear_which_implies_wit_1.
